<?xml version="1.0"?>
<rdf:RDF xmlns="http://siemens.com/knowledge_graph/cyber_physical_systems/industrial_cps_df#"
     xml:base="http://siemens.com/knowledge_graph/cyber_physical_systems/industrial_cps_df"
     xmlns:schema="http://schema.org/"
     xmlns:df="http://siemens.com/knowledge_graph/cyber_physical_systems/industrial_cps_df#"
     xmlns:rdf="http://www.w3.org/1999/02/22-rdf-syntax-ns#"
     xmlns:owl="http://www.w3.org/2002/07/owl#"
     xmlns:xml="http://www.w3.org/XML/1998/namespace"
     xmlns:xsd="http://www.w3.org/2001/XMLSchema#"
     xmlns:rdfs="http://www.w3.org/2000/01/rdf-schema#"
     xmlns:dc="http://purl.org/dc/elements/1.1/">
    <owl:Ontology rdf:about="http://siemens.com/knowledge_graph/cyber_physical_systems/industrial_cps_df">
        <owl:imports rdf:resource="http://siemens.com/knowledge_graph/cyber_physical_systems/industrial_cps"/>
        <rdfs:comment>Ontology for Discrete Manufacturing in Industrial Cyber-Physical Systems (CPS)</rdfs:comment>
        <rdfs:label>Industrial CPS DF Ontology</rdfs:label>
    </owl:Ontology>
    


    <!-- 
    ///////////////////////////////////////////////////////////////////////////////////////
    //
    // Annotation properties
    //
    ///////////////////////////////////////////////////////////////////////////////////////
     -->

    


    <!-- http://siemens.com/knowledge_graph/cyber_physical_systems/industrial_cps_df#processConstraint -->

    <owl:AnnotationProperty rdf:about="http://siemens.com/knowledge_graph/cyber_physical_systems/industrial_cps_df#processConstraint">
        <rdfs:comment>processConstraint is an annotation property which contains one constraint on a Process as string.
It is encoded in the following way:
##id##: idValue ##expr##: exprValue

Neither comma nor colon may be part of the values, otherwise we have to rethink the encoding.</rdfs:comment>
        <rdfs:label>process constraint</rdfs:label>
        <rdfs:range rdf:resource="http://www.w3.org/2001/XMLSchema#string"/>
        <rdfs:domain rdf:resource="http://siemens.com/knowledge_graph/cyber_physical_systems/industrial_cps#Process"/>
    </owl:AnnotationProperty>
    


    <!-- http://siemens.com/knowledge_graph/cyber_physical_systems/industrial_cps_df#processConstraintSolverAttr -->

    <owl:AnnotationProperty rdf:about="http://siemens.com/knowledge_graph/cyber_physical_systems/industrial_cps_df#processConstraintSolverAttr">
        <rdfs:comment>processConstraintSolverAttr is an annotation property which contains one constraint of an offered skill as string.
It is encoded in the following way:
##id##: idValue ##expr##: exprType:exprValue

Example:
##id##: canInsertIntoGap ##expr##: Boolean:True

It supports the following types: String, Integer, Double and Boolean.

Remark:
This looks similar to the processConstraint but has the additional type field.Therefore we have decided to make a second property so we don&apos;t need to touch the working code for processConstraint.
Later on we can rethink if we should merge these two properties.</rdfs:comment>
        <rdfs:label>process ConstraintSolver Attribute</rdfs:label>
    </owl:AnnotationProperty>
    


    <!-- 
    ///////////////////////////////////////////////////////////////////////////////////////
    //
    // Object Properties
    //
    ///////////////////////////////////////////////////////////////////////////////////////
     -->

    


    <!-- http://siemens.com/knowledge_graph/cyber_physical_systems/industrial_cps_df#materialType -->

    <owl:ObjectProperty rdf:about="http://siemens.com/knowledge_graph/cyber_physical_systems/industrial_cps_df#materialType">
        <rdfs:domain rdf:resource="http://siemens.com/knowledge_graph/cyber_physical_systems/industrial_cps#Material"/>
        <rdfs:range rdf:resource="http://siemens.com/knowledge_graph/cyber_physical_systems/industrial_cps_df#MaterialType"/>
        <rdfs:comment>materialType assigns its material type to a certain material object.</rdfs:comment>
        <rdfs:label>materialType</rdfs:label>
    </owl:ObjectProperty>
    


    <!-- http://siemens.com/knowledge_graph/industrial_upper_ontology#isPartOf -->

    <owl:ObjectProperty rdf:about="http://siemens.com/knowledge_graph/industrial_upper_ontology#isPartOf">
        <owl:inverseOf>
            <rdf:Description>
                <owl:inverseOf rdf:resource="http://siemens.com/knowledge_graph/industrial_upper_ontology#isPartOf"/>
            </rdf:Description>
        </owl:inverseOf>
    </owl:ObjectProperty>
    


    <!-- 
    ///////////////////////////////////////////////////////////////////////////////////////
    //
    // Data properties
    //
    ///////////////////////////////////////////////////////////////////////////////////////
     -->

    


    <!-- http://siemens.com/knowledge_graph/cyber_physical_systems/industrial_cps_df#height -->

    <owl:DatatypeProperty rdf:about="http://siemens.com/knowledge_graph/cyber_physical_systems/industrial_cps_df#height">
        <rdfs:subPropertyOf rdf:resource="http://siemens.com/knowledge_graph/industrial_upper_ontology#attribute"/>
        <rdfs:comment>height (in mm)</rdfs:comment>
        <rdfs:label>height (in mm)</rdfs:label>
    </owl:DatatypeProperty>
    


    <!-- http://siemens.com/knowledge_graph/cyber_physical_systems/industrial_cps_df#width -->

    <owl:DatatypeProperty rdf:about="http://siemens.com/knowledge_graph/cyber_physical_systems/industrial_cps_df#width">
        <rdfs:subPropertyOf rdf:resource="http://siemens.com/knowledge_graph/industrial_upper_ontology#attribute"/>
        <rdf:type rdf:resource="http://www.w3.org/2002/07/owl#FunctionalProperty"/>
        <rdfs:domain rdf:resource="http://siemens.com/knowledge_graph/cyber_physical_systems/industrial_cps_df#Workpiece"/>
        <rdfs:range rdf:resource="http://www.w3.org/2001/XMLSchema#integer"/>
        <rdfs:comment>width (in mm)</rdfs:comment>
        <rdfs:label>width (in mm)</rdfs:label>
    </owl:DatatypeProperty>
    


    <!-- http://siemens.com/knowledge_graph/industrial_upper_ontology#attribute -->

    <owl:DatatypeProperty rdf:about="http://siemens.com/knowledge_graph/industrial_upper_ontology#attribute"/>
    


    <!-- 
    ///////////////////////////////////////////////////////////////////////////////////////
    //
    // Classes
    //
    ///////////////////////////////////////////////////////////////////////////////////////
     -->

    


    <!-- http://siemens.com/knowledge_graph/cyber_physical_systems/industrial_cps#Machinery -->

    <owl:Class rdf:about="http://siemens.com/knowledge_graph/cyber_physical_systems/industrial_cps#Machinery"/>
    


    <!-- http://siemens.com/knowledge_graph/cyber_physical_systems/industrial_cps#Material -->

    <owl:Class rdf:about="http://siemens.com/knowledge_graph/cyber_physical_systems/industrial_cps#Material"/>
    


    <!-- http://siemens.com/knowledge_graph/cyber_physical_systems/industrial_cps#Process -->

    <owl:Class rdf:about="http://siemens.com/knowledge_graph/cyber_physical_systems/industrial_cps#Process"/>
    


    <!-- http://siemens.com/knowledge_graph/cyber_physical_systems/industrial_cps_df#Assembling -->

    <owl:Class rdf:about="http://siemens.com/knowledge_graph/cyber_physical_systems/industrial_cps_df#Assembling">
        <rdfs:subClassOf rdf:resource="http://siemens.com/knowledge_graph/cyber_physical_systems/industrial_cps_df#Joining"/>
        <rdfs:comment>Placing workpieces together; DIN 8593 (4.1)</rdfs:comment>
        <rdfs:label>Assembling</rdfs:label>
    </owl:Class>
    


    <!-- http://siemens.com/knowledge_graph/cyber_physical_systems/industrial_cps_df#Assembly -->

    <owl:Class rdf:about="http://siemens.com/knowledge_graph/cyber_physical_systems/industrial_cps_df#Assembly">
        <rdfs:subClassOf rdf:resource="http://siemens.com/knowledge_graph/cyber_physical_systems/industrial_cps_df#Workpiece"/>
        <rdfs:label>Assembly</rdfs:label>
    </owl:Class>
    


    <!-- http://siemens.com/knowledge_graph/cyber_physical_systems/industrial_cps_df#AtomicWorkpiece -->

    <owl:Class rdf:about="http://siemens.com/knowledge_graph/cyber_physical_systems/industrial_cps_df#AtomicWorkpiece">
        <rdfs:subClassOf rdf:resource="http://siemens.com/knowledge_graph/cyber_physical_systems/industrial_cps_df#Workpiece"/>
        <rdfs:label>AtomicWorkpiece</rdfs:label>
    </owl:Class>
    


    <!-- http://siemens.com/knowledge_graph/cyber_physical_systems/industrial_cps_df#Charging -->

    <owl:Class rdf:about="http://siemens.com/knowledge_graph/cyber_physical_systems/industrial_cps_df#Charging">
        <rdfs:subClassOf rdf:resource="http://siemens.com/knowledge_graph/cyber_physical_systems/industrial_cps_df#Moving"/>
        <owl:disjointWith rdf:resource="http://siemens.com/knowledge_graph/cyber_physical_systems/industrial_cps_df#Feeding"/>
        <owl:disjointWith rdf:resource="http://siemens.com/knowledge_graph/cyber_physical_systems/industrial_cps_df#Transporting"/>
        <owl:disjointWith rdf:resource="http://siemens.com/knowledge_graph/cyber_physical_systems/industrial_cps_df#Turning"/>
        <owl:disjointWith rdf:resource="http://siemens.com/knowledge_graph/cyber_physical_systems/industrial_cps_df#Unfeeding"/>
        <rdfs:comment>Charging means the preparation of a workpiece for being worked on, e.g. the placing on a carrier for moving it through a production line. (VDI 2860)</rdfs:comment>
        <rdfs:label>Charging</rdfs:label>
    </owl:Class>
    <owl:Axiom>
        <owl:annotatedSource rdf:resource="http://siemens.com/knowledge_graph/cyber_physical_systems/industrial_cps_df#Charging"/>
        <owl:annotatedProperty rdf:resource="http://www.w3.org/2000/01/rdf-schema#subClassOf"/>
        <owl:annotatedTarget rdf:resource="http://siemens.com/knowledge_graph/cyber_physical_systems/industrial_cps_df#Moving"/>
        <rdfs:comment>Feeding some workpiece into a production line (VDI2860)</rdfs:comment>
    </owl:Axiom>
    


    <!-- http://siemens.com/knowledge_graph/cyber_physical_systems/industrial_cps_df#Chipping -->

    <owl:Class rdf:about="http://siemens.com/knowledge_graph/cyber_physical_systems/industrial_cps_df#Chipping">
        <rdfs:subClassOf rdf:resource="http://siemens.com/knowledge_graph/cyber_physical_systems/industrial_cps_df#Separating"/>
        <owl:disjointWith rdf:resource="http://siemens.com/knowledge_graph/cyber_physical_systems/industrial_cps_df#Disassembling"/>
        <rdfs:comment>Chipping away bits of material from a solid block. Produces waste. According to DIN 8591 (German: Spanen)</rdfs:comment>
        <rdfs:label>Chipping</rdfs:label>
    </owl:Class>
    


    <!-- http://siemens.com/knowledge_graph/cyber_physical_systems/industrial_cps_df#Disassembling -->

    <owl:Class rdf:about="http://siemens.com/knowledge_graph/cyber_physical_systems/industrial_cps_df#Disassembling">
        <rdfs:subClassOf rdf:resource="http://siemens.com/knowledge_graph/cyber_physical_systems/industrial_cps_df#Separating"/>
        <rdfs:comment>According to DIN 8580 3.5</rdfs:comment>
        <rdfs:label>Disassembling</rdfs:label>
    </owl:Class>
    


    <!-- http://siemens.com/knowledge_graph/cyber_physical_systems/industrial_cps_df#Dismantling -->

    <owl:Class rdf:about="http://siemens.com/knowledge_graph/cyber_physical_systems/industrial_cps_df#Dismantling">
        <rdfs:subClassOf rdf:resource="http://siemens.com/knowledge_graph/cyber_physical_systems/industrial_cps_df#Disassembling"/>
        <rdfs:comment>Dismantling, according to DIN 8591 3.5.1, is (1) the separation of previously joined work pieces of geometrically defined forms or (2) the separation of work pieces of geometrically defined forms and filled shapeless substances. No damaging of the work pieces is allowed. [source: https://books.google.de/books?id=0D_c3OBobdYC&amp;pg=PA7&amp;lpg=PA7&amp;dq=DIN+8591+disassembling&amp;source=bl&amp;ots=9SBONVefaG&amp;sig=FVlel8JKse9vpqPosASOB9JTEQ8&amp;hl=de&amp;sa=X&amp;ved=0ahUKEwiWoY-rhtLYAhWEliwKHaUYCDAQ6AEINzAD#v=onepage&amp;q=DIN%208591%20disassembling&amp;f=false]</rdfs:comment>
        <rdfs:label>Dismantling</rdfs:label>
    </owl:Class>
    <owl:Axiom>
        <owl:annotatedSource rdf:resource="http://siemens.com/knowledge_graph/cyber_physical_systems/industrial_cps_df#Dismantling"/>
        <owl:annotatedProperty rdf:resource="http://www.w3.org/2000/01/rdf-schema#subClassOf"/>
        <owl:annotatedTarget rdf:resource="http://siemens.com/knowledge_graph/cyber_physical_systems/industrial_cps_df#Disassembling"/>
        <rdfs:comment>performs dismantling (according to DIN 8591 3.5.1)</rdfs:comment>
    </owl:Axiom>
    


    <!-- http://siemens.com/knowledge_graph/cyber_physical_systems/industrial_cps_df#Feeding -->

    <owl:Class rdf:about="http://siemens.com/knowledge_graph/cyber_physical_systems/industrial_cps_df#Feeding">
        <rdfs:subClassOf rdf:resource="http://siemens.com/knowledge_graph/cyber_physical_systems/industrial_cps_df#Moving"/>
        <owl:disjointWith rdf:resource="http://siemens.com/knowledge_graph/cyber_physical_systems/industrial_cps_df#Transporting"/>
        <owl:disjointWith rdf:resource="http://siemens.com/knowledge_graph/cyber_physical_systems/industrial_cps_df#Turning"/>
        <owl:disjointWith rdf:resource="http://siemens.com/knowledge_graph/cyber_physical_systems/industrial_cps_df#Unfeeding"/>
        <rdfs:comment>Supplying workpieces into a production system. Synonym to Feeding.</rdfs:comment>
        <rdfs:label>Supplying</rdfs:label>
    </owl:Class>
    


    <!-- http://siemens.com/knowledge_graph/cyber_physical_systems/industrial_cps_df#Fixating -->

    <owl:Class rdf:about="http://siemens.com/knowledge_graph/cyber_physical_systems/industrial_cps_df#Fixating">
        <rdfs:subClassOf rdf:resource="http://siemens.com/knowledge_graph/cyber_physical_systems/industrial_cps_df#Handling"/>
        <owl:disjointWith rdf:resource="http://siemens.com/knowledge_graph/cyber_physical_systems/industrial_cps_df#Moving"/>
        <owl:disjointWith rdf:resource="http://siemens.com/knowledge_graph/cyber_physical_systems/industrial_cps_df#Packaging"/>
        <owl:disjointWith rdf:resource="http://siemens.com/knowledge_graph/cyber_physical_systems/industrial_cps_df#Storing"/>
        <rdfs:comment>Fixating a workpiece into a fixture.</rdfs:comment>
        <rdfs:label>Fixating</rdfs:label>
    </owl:Class>
    


    <!-- http://siemens.com/knowledge_graph/cyber_physical_systems/industrial_cps_df#Forming -->

    <owl:Class rdf:about="http://siemens.com/knowledge_graph/cyber_physical_systems/industrial_cps_df#Forming">
        <rdfs:subClassOf rdf:resource="http://siemens.com/knowledge_graph/cyber_physical_systems/industrial_cps_df#Manufacturing"/>
        <owl:disjointWith rdf:resource="http://siemens.com/knowledge_graph/cyber_physical_systems/industrial_cps_df#Joining"/>
        <owl:disjointWith rdf:resource="http://siemens.com/knowledge_graph/cyber_physical_systems/industrial_cps_df#Separating"/>
        <rdfs:comment>According to DIN 85xx group 2</rdfs:comment>
        <rdfs:label>Forming</rdfs:label>
    </owl:Class>
    


    <!-- http://siemens.com/knowledge_graph/cyber_physical_systems/industrial_cps_df#Handling -->

    <owl:Class rdf:about="http://siemens.com/knowledge_graph/cyber_physical_systems/industrial_cps_df#Handling">
        <rdfs:subClassOf rdf:resource="http://siemens.com/knowledge_graph/cyber_physical_systems/industrial_cps#Process"/>
        <owl:disjointWith rdf:resource="http://siemens.com/knowledge_graph/cyber_physical_systems/industrial_cps_df#Manufacturing"/>
        <rdfs:comment>Handling of material in production (e.g. transportation etc.); according to VDI 2860</rdfs:comment>
        <rdfs:label>Handling</rdfs:label>
    </owl:Class>
    


    <!-- http://siemens.com/knowledge_graph/cyber_physical_systems/industrial_cps_df#Inserting -->

    <owl:Class rdf:about="http://siemens.com/knowledge_graph/cyber_physical_systems/industrial_cps_df#Inserting">
        <rdfs:subClassOf rdf:resource="http://siemens.com/knowledge_graph/cyber_physical_systems/industrial_cps_df#Assembling"/>
        <owl:disjointWith rdf:resource="http://siemens.com/knowledge_graph/cyber_physical_systems/industrial_cps_df#PlacingOnTop"/>
        <owl:disjointWith rdf:resource="http://siemens.com/knowledge_graph/cyber_physical_systems/industrial_cps_df#Shunting"/>
        <owl:disjointWith rdf:resource="http://siemens.com/knowledge_graph/cyber_physical_systems/industrial_cps_df#SpreadFitting"/>
        <rdfs:comment>Inserting a workpiece loosely into another one; DIN 8593-1 (4.1.2)</rdfs:comment>
        <rdfs:label>Inserting</rdfs:label>
    </owl:Class>
    <owl:Axiom>
        <owl:annotatedSource rdf:resource="http://siemens.com/knowledge_graph/cyber_physical_systems/industrial_cps_df#Inserting"/>
        <owl:annotatedProperty rdf:resource="http://www.w3.org/2000/01/rdf-schema#subClassOf"/>
        <owl:annotatedTarget rdf:resource="http://siemens.com/knowledge_graph/cyber_physical_systems/industrial_cps_df#Assembling"/>
        <rdfs:comment>applies inserting (according to DIN 8593)</rdfs:comment>
    </owl:Axiom>
    


    <!-- http://siemens.com/knowledge_graph/cyber_physical_systems/industrial_cps_df#Joining -->

    <owl:Class rdf:about="http://siemens.com/knowledge_graph/cyber_physical_systems/industrial_cps_df#Joining">
        <rdfs:subClassOf rdf:resource="http://siemens.com/knowledge_graph/cyber_physical_systems/industrial_cps_df#Manufacturing"/>
        <owl:disjointWith rdf:resource="http://siemens.com/knowledge_graph/cyber_physical_systems/industrial_cps_df#Separating"/>
        <rdfs:comment>Joining of workpieces to assemblies in production; joiningmethods acording to DIN 8593 group 4

Remark:
removed the superclass &quot;cps:canAffectResultingMaterial only ( inverse (iuo:isPartOf) some owl:Thing)&quot; because we don&apos;t have the property &quot;canAffectResultingMaterial&quot; anymore.</rdfs:comment>
        <rdfs:label>Joining</rdfs:label>
    </owl:Class>
    


    <!-- http://siemens.com/knowledge_graph/cyber_physical_systems/industrial_cps_df#Manufacturing -->

    <owl:Class rdf:about="http://siemens.com/knowledge_graph/cyber_physical_systems/industrial_cps_df#Manufacturing">
        <rdfs:subClassOf rdf:resource="http://siemens.com/knowledge_graph/cyber_physical_systems/industrial_cps#Process"/>
        <rdfs:comment>Manufacturing methods according to DIN 85xx (see also https://www.co2pe.org/?Taxonomy)</rdfs:comment>
        <rdfs:label>Manufacturing</rdfs:label>
    </owl:Class>
    


    <!-- http://siemens.com/knowledge_graph/cyber_physical_systems/industrial_cps_df#MaterialType -->

    <owl:Class rdf:about="http://siemens.com/knowledge_graph/cyber_physical_systems/industrial_cps_df#MaterialType">
        <rdfs:subClassOf rdf:resource="http://siemens.com/knowledge_graph/industrial_upper_ontology#InformationObject"/>
        <rdfs:comment>Material Type denotes the substance or matter of a material.

e.g. Glass, Metal, Plastic.

We have decided not only to distinguish different material types by names but to provide real objects for this which may later on allow for more complex representations, e.g. chemical mix of some plastic or metal or quality values for strength, flexibility etc.</rdfs:comment>
        <rdfs:label>Material Type</rdfs:label>
    </owl:Class>
    


    <!-- http://siemens.com/knowledge_graph/cyber_physical_systems/industrial_cps_df#Moving -->

    <owl:Class rdf:about="http://siemens.com/knowledge_graph/cyber_physical_systems/industrial_cps_df#Moving">
        <rdfs:subClassOf rdf:resource="http://siemens.com/knowledge_graph/cyber_physical_systems/industrial_cps_df#Handling"/>
        <owl:disjointWith rdf:resource="http://siemens.com/knowledge_graph/cyber_physical_systems/industrial_cps_df#Packaging"/>
        <owl:disjointWith rdf:resource="http://siemens.com/knowledge_graph/cyber_physical_systems/industrial_cps_df#Storing"/>
        <rdfs:comment>The generic moving property.</rdfs:comment>
        <rdfs:label>Moving</rdfs:label>
    </owl:Class>
    


    <!-- http://siemens.com/knowledge_graph/cyber_physical_systems/industrial_cps_df#Packaging -->

    <owl:Class rdf:about="http://siemens.com/knowledge_graph/cyber_physical_systems/industrial_cps_df#Packaging">
        <rdfs:subClassOf rdf:resource="http://siemens.com/knowledge_graph/cyber_physical_systems/industrial_cps_df#Handling"/>
        <owl:disjointWith rdf:resource="http://siemens.com/knowledge_graph/cyber_physical_systems/industrial_cps_df#Storing"/>
        <rdfs:comment>Packaging is the process of  preparing the product for transport/sale etc. The packaging ensures that the product will remain intact and is presented in a nice way.</rdfs:comment>
        <rdfs:label>Packaging</rdfs:label>
    </owl:Class>
    


    <!-- http://siemens.com/knowledge_graph/cyber_physical_systems/industrial_cps_df#Picking -->

    <owl:Class rdf:about="http://siemens.com/knowledge_graph/cyber_physical_systems/industrial_cps_df#Picking">
        <rdfs:subClassOf rdf:resource="http://siemens.com/knowledge_graph/cyber_physical_systems/industrial_cps_df#Handling"/>
        <rdfs:comment>Picking a workpiece.</rdfs:comment>
        <rdfs:label>Picking</rdfs:label>
    </owl:Class>
    


    <!-- http://siemens.com/knowledge_graph/cyber_physical_systems/industrial_cps_df#Placing -->

    <owl:Class rdf:about="http://siemens.com/knowledge_graph/cyber_physical_systems/industrial_cps_df#Placing">
        <rdfs:subClassOf rdf:resource="http://siemens.com/knowledge_graph/cyber_physical_systems/industrial_cps_df#Handling"/>
        <rdfs:comment> Placing a workpiece onto a surface position.</rdfs:comment>
        <rdfs:label>Placing</rdfs:label>
    </owl:Class>
    


    <!-- http://siemens.com/knowledge_graph/cyber_physical_systems/industrial_cps_df#PlacingOnTop -->

    <owl:Class rdf:about="http://siemens.com/knowledge_graph/cyber_physical_systems/industrial_cps_df#PlacingOnTop">
        <rdfs:subClassOf rdf:resource="http://siemens.com/knowledge_graph/cyber_physical_systems/industrial_cps_df#Assembling"/>
        <rdfs:comment>Placing a workpiece loosely on top of some other workpiece; DIN 8593-1 (4.1.1)</rdfs:comment>
        <rdfs:label>Placing on top</rdfs:label>
    </owl:Class>
    


    <!-- http://siemens.com/knowledge_graph/cyber_physical_systems/industrial_cps_df#Punching -->

    <owl:Class rdf:about="http://siemens.com/knowledge_graph/cyber_physical_systems/industrial_cps_df#Punching">
        <rdfs:subClassOf rdf:resource="http://siemens.com/knowledge_graph/cyber_physical_systems/industrial_cps_df#Chipping"/>
        <rdfs:comment>Punching into solid block (e.g. engraving of signature into a metal plate); According to DIN 8591 (German: Stanzen/Hobeln?)</rdfs:comment>
        <rdfs:label>Punching</rdfs:label>
    </owl:Class>
    <owl:Axiom>
        <owl:annotatedSource rdf:resource="http://siemens.com/knowledge_graph/cyber_physical_systems/industrial_cps_df#Punching"/>
        <owl:annotatedProperty rdf:resource="http://www.w3.org/2000/01/rdf-schema#subClassOf"/>
        <owl:annotatedTarget rdf:resource="http://siemens.com/knowledge_graph/cyber_physical_systems/industrial_cps_df#Chipping"/>
        <rdfs:comment>performs punching (according to DIN 8591 3.2.x)</rdfs:comment>
    </owl:Axiom>
    


    <!-- http://siemens.com/knowledge_graph/cyber_physical_systems/industrial_cps_df#Separating -->

    <owl:Class rdf:about="http://siemens.com/knowledge_graph/cyber_physical_systems/industrial_cps_df#Separating">
        <rdfs:subClassOf rdf:resource="http://siemens.com/knowledge_graph/cyber_physical_systems/industrial_cps_df#Manufacturing"/>
        <rdfs:comment>Separating assemblies into their original parts; methods acording to DIN 8593 group 3</rdfs:comment>
        <rdfs:label>Separation</rdfs:label>
    </owl:Class>
    


    <!-- http://siemens.com/knowledge_graph/cyber_physical_systems/industrial_cps_df#Shunting -->

    <owl:Class rdf:about="http://siemens.com/knowledge_graph/cyber_physical_systems/industrial_cps_df#Shunting">
        <rdfs:subClassOf rdf:resource="http://siemens.com/knowledge_graph/cyber_physical_systems/industrial_cps_df#Assembling"/>
        <rdfs:comment>joining two pieces by sliding a moving piece into or onto the target piece according to DIN 8395 (4.1.3)</rdfs:comment>
        <rdfs:label>Shunting</rdfs:label>
    </owl:Class>
    


    <!-- http://siemens.com/knowledge_graph/cyber_physical_systems/industrial_cps_df#SpreadFitting -->

    <owl:Class rdf:about="http://siemens.com/knowledge_graph/cyber_physical_systems/industrial_cps_df#SpreadFitting">
        <rdfs:subClassOf rdf:resource="http://siemens.com/knowledge_graph/cyber_physical_systems/industrial_cps_df#Assembling"/>
        <rdfs:comment>joins two pieces by pressing a moving piece onto a target piece with force according to DIN 8593 (4.1.6); the moving piece is first deformed and then snaps back into its original form, which yields a stable connection</rdfs:comment>
        <rdfs:label>SpreadFitting</rdfs:label>
    </owl:Class>
    


    <!-- http://siemens.com/knowledge_graph/cyber_physical_systems/industrial_cps_df#Storing -->

    <owl:Class rdf:about="http://siemens.com/knowledge_graph/cyber_physical_systems/industrial_cps_df#Storing">
        <rdfs:subClassOf rdf:resource="http://siemens.com/knowledge_graph/cyber_physical_systems/industrial_cps_df#Handling"/>
        <rdfs:comment>Storing workpieces on a material handling system (not in VDI 2860!?)</rdfs:comment>
        <rdfs:label>Storing</rdfs:label>
    </owl:Class>
    


    <!-- http://siemens.com/knowledge_graph/cyber_physical_systems/industrial_cps_df#Transporting -->

    <owl:Class rdf:about="http://siemens.com/knowledge_graph/cyber_physical_systems/industrial_cps_df#Transporting">
        <rdfs:subClassOf rdf:resource="http://siemens.com/knowledge_graph/cyber_physical_systems/industrial_cps_df#Moving"/>
        <owl:disjointWith rdf:resource="http://siemens.com/knowledge_graph/cyber_physical_systems/industrial_cps_df#Turning"/>
        <owl:disjointWith rdf:resource="http://siemens.com/knowledge_graph/cyber_physical_systems/industrial_cps_df#Unfeeding"/>
        <rdfs:comment>Transporting material</rdfs:comment>
        <rdfs:label>Transporting</rdfs:label>
    </owl:Class>
    


    <!-- http://siemens.com/knowledge_graph/cyber_physical_systems/industrial_cps_df#Turning -->

    <owl:Class rdf:about="http://siemens.com/knowledge_graph/cyber_physical_systems/industrial_cps_df#Turning">
        <rdfs:subClassOf rdf:resource="http://siemens.com/knowledge_graph/cyber_physical_systems/industrial_cps_df#Moving"/>
        <owl:disjointWith rdf:resource="http://siemens.com/knowledge_graph/cyber_physical_systems/industrial_cps_df#Unfeeding"/>
        <rdfs:comment>Turning changes the orientation of a workpiece/product.</rdfs:comment>
        <rdfs:label>Turning</rdfs:label>
    </owl:Class>
    


    <!-- http://siemens.com/knowledge_graph/cyber_physical_systems/industrial_cps_df#Unfeeding -->

    <owl:Class rdf:about="http://siemens.com/knowledge_graph/cyber_physical_systems/industrial_cps_df#Unfeeding">
        <rdfs:subClassOf rdf:resource="http://siemens.com/knowledge_graph/cyber_physical_systems/industrial_cps_df#Moving"/>
        <rdfs:comment>Unfeeding (taking out) of material from a production system, according to VDI 2860 (German: Ausgeben)</rdfs:comment>
        <rdfs:label>Unfeeding</rdfs:label>
    </owl:Class>
    <owl:Axiom>
        <owl:annotatedSource rdf:resource="http://siemens.com/knowledge_graph/cyber_physical_systems/industrial_cps_df#Unfeeding"/>
        <owl:annotatedProperty rdf:resource="http://www.w3.org/2000/01/rdf-schema#subClassOf"/>
        <owl:annotatedTarget rdf:resource="http://siemens.com/knowledge_graph/cyber_physical_systems/industrial_cps_df#Moving"/>
        <rdfs:comment>Unfeeding (taking out) of material from a production system (VDI 2860)</rdfs:comment>
    </owl:Axiom>
    


    <!-- http://siemens.com/knowledge_graph/cyber_physical_systems/industrial_cps_df#Workpiece -->

    <owl:Class rdf:about="http://siemens.com/knowledge_graph/cyber_physical_systems/industrial_cps_df#Workpiece">
        <rdfs:subClassOf rdf:resource="http://siemens.com/knowledge_graph/cyber_physical_systems/industrial_cps#Material"/>
        <rdfs:comment>A Workpiece is a piece of material which can be handled with discrete manufacturing.</rdfs:comment>
        <rdfs:label>Workpiece</rdfs:label>
    </owl:Class>
    


    <!-- http://siemens.com/knowledge_graph/industrial_upper_ontology#InformationObject -->

    <owl:Class rdf:about="http://siemens.com/knowledge_graph/industrial_upper_ontology#InformationObject"/>
</rdf:RDF>



<!-- Generated by the OWL API (version 4.2.8.20170104-2310) https://github.com/owlcs/owlapi -->

